messageInvariantPrototypes/paxos/decentralizedMonotonicTemplated/applicationProof.dfy
@@ -78,7 +78,7 @@ ghost predicate OneValuePerBallotLeaderAndLearners(c: Constants, v: Variables)
     && c.ValidLearnerIdx(lnr)
     && VB(acceptedVal, ldr) in v.History(i).learners[lnr].receivedAccepts.m
   ::
-    acceptedVal == v.History(i).leaders[ldr].value
+    acceptedVal == v.History(i).leaders[ldr].Value()
 }
 
 // Leaders and Acceptors only have one value for each ballot
@@ -91,7 +91,7 @@ ghost predicate OneValuePerBallotLeaderAndAcceptors(c: Constants, v: Variables)
     && c.ValidAcceptorIdx(acc)
     && v.History(i).acceptors[acc].HasAccepted(VB(acceptedVal, ldr))
   ::
-    acceptedVal == v.History(i).leaders[ldr].value
+    acceptedVal == v.History(i).leaders[ldr].Value()
 }
 
 // Learner's receivedAccepts contain valid acceptor ids
@@ -143,7 +143,7 @@ ghost predicate LearnerReceivedAcceptImpliesProposed(c: Constants, v: Variables)
     && vb in v.History(i).learners[lnr].receivedAccepts.m
   ::
     && v.History(i).LeaderCanPropose(c, vb.b)
-    && v.History(i).leaders[vb.b].value == vb.v
+    && v.History(i).leaders[vb.b].Value() == vb.v
 }
 
 
@@ -191,7 +191,7 @@ ghost predicate AcceptorAcceptedImpliesProposed(c: Constants, v: Variables)
   ::
     var vb := v.History(i).acceptors[acc].acceptedVB.value;
     && v.History(i).LeaderCanPropose(c, vb.b)
-    && v.History(i).leaders[vb.b].value == vb.v
+    && v.History(i).leaders[vb.b].Value() == vb.v
 }
 
 ghost predicate LeaderValidReceivedPromises(c: Constants, v: Variables)
@@ -200,7 +200,7 @@ ghost predicate LeaderValidReceivedPromises(c: Constants, v: Variables)
   forall ldr, acc, i | 
     && v.ValidHistoryIdx(i)
     && c.ValidLeaderIdx(ldr)
-    && acc in v.History(i).leaders[ldr].receivedPromises.s
+    && acc in v.History(i).leaders[ldr].ReceivedPromises()
   ::
     c.ValidAcceptorIdx(acc)
 }
@@ -232,10 +232,10 @@ ghost predicate LeaderHearedImpliesProposed(c: Constants, v: Variables)
     var b := vi.leaders[ldr].highestHeardBallot.value;
     && c.ValidLeaderIdx(b)
     && vi.LeaderCanPropose(c, b)
-    && vi.leaders[b].value == vi.leaders[ldr].value
+    && vi.leaders[b].Value() == vi.leaders[ldr].Value()
 }
 
-// For all ldr, acc such that acc in ldr.receivedPromises.s, acc's current promise
+// For all ldr, acc such that acc in ldr.ReceivedPromises(), acc's current promise
 // must be >= ldr's ballot
 ghost predicate LeaderReceivedPromisesImpliesAcceptorState(c: Constants, v: Variables)
   requires v.WF(c)
@@ -244,7 +244,7 @@ ghost predicate LeaderReceivedPromisesImpliesAcceptorState(c: Constants, v: Vari
     && v.ValidHistoryIdx(i)
     && c.ValidLeaderIdx(ldr)
     && c.ValidAcceptorIdx(acc)
-    && acc in v.History(i).leaders[ldr].receivedPromises.s
+    && acc in v.History(i).leaders[ldr].ReceivedPromises()
   ::
     v.History(i).acceptors[acc].HasPromisedAtLeast(ldr)
 }
@@ -262,7 +262,7 @@ ghost predicate LeaderHighestHeardToPromisedRangeHasNoAccepts(c: Constants, v: V
     && vb in v.History(i).learners[lnr].receivedAccepts.m
     && vb.b < ldr
     && v.History(i).leaders[ldr].HeardAtMost(vb.b)
-    && acc in v.History(i).leaders[ldr].receivedPromises.s
+    && acc in v.History(i).leaders[ldr].ReceivedPromises()
   ::
     acc !in v.History(i).learners[lnr].receivedAccepts.m[vb]
 }
@@ -304,7 +304,7 @@ ghost predicate ChosenValImpliesLeaderOnlyHearsVal(c: Constants, v: Variables)
     && c.ValidLeaderIdx(ldrBal)
     && v.History(i).leaders[ldrBal].HeardAtLeast(vb.b)
   ::
-    v.History(i).leaders[ldrBal].value == vb.v
+    v.History(i).leaders[ldrBal].Value() == vb.v
 }
 
 // Application bundle
@@ -456,8 +456,7 @@ lemma InvNextOneValuePerBallotAcceptorsAndLearners(c: Constants, v: Variables, v
   requires ValidMessageSrc(c, v) && ValidMessageSrc(c, v')
   requires SendProposeValidity(c, v) && SendProposeValidity(c, v')
   requires SendAcceptValidity(c, v) && SendAcceptValidity(c, v')
-  requires LeaderReceivedPromisesMonotonic(c, v)
-  requires LeaderCanProposeVMonotonic(c, v)
+  requires LeaderReceivedPromisesAndValueMonotonic(c, v)
   requires LearnerReceivedAcceptsMonotonic(c, v')
   requires OneValuePerBallot(c, v)
   requires AcceptorValidPromisedAndAccepted(c, v) // prereq for AcceptorAcceptedImpliesProposed
@@ -506,8 +505,7 @@ lemma InvNextOneValuePerBallotAcceptorsAndLearners(c: Constants, v: Variables, v
 lemma InvNextOneValuePerBallotLeaderAndLearners(c: Constants, v: Variables, v': Variables)
   requires Inv(c, v) && v'.WF(c)
   requires ValidMessageSrc(c, v) && ValidMessageSrc(c, v')
-  requires LeaderReceivedPromisesMonotonic(c, v')
-  requires LeaderCanProposeVMonotonic(c, v')
+  requires LeaderReceivedPromisesAndValueMonotonic(c, v')
   requires Next(c, v, v')
   ensures OneValuePerBallotLeaderAndLearners(c, v')
 {
@@ -517,7 +515,7 @@ lemma InvNextOneValuePerBallotLeaderAndLearners(c: Constants, v: Variables, v': 
     && c.ValidLearnerIdx(lnr)
     && VB(acceptedVal, ldr) in v'.History(i).learners[lnr].receivedAccepts.m
   ensures
-    acceptedVal == v'.History(i).leaders[ldr].value
+    acceptedVal == v'.History(i).leaders[ldr].Value()
   {
     VariableNextProperties(c, v, v');
     LeaderCanProposeMonotonicLemma(c, v');
@@ -541,7 +539,7 @@ lemma InvNextOneValuePerBallotLeaderAndAcceptors(c: Constants, v: Variables, v':
     && c.ValidAcceptorIdx(acc)
     && v'.History(i).acceptors[acc].HasAccepted(VB(acceptedVal, ldr))
   ensures
-    acceptedVal == v'.History(i).leaders[ldr].value
+    acceptedVal == v'.History(i).leaders[ldr].Value()
   {
     VariableNextProperties(c, v, v');
     if i == |v'.history| - 1 {
@@ -554,7 +552,7 @@ lemma InvNextOneValuePerBallotLeaderAndAcceptors(c: Constants, v: Variables, v':
           // triggers
           var step :| AcceptorHost.NextStep(ac, ah, ah', step, msgOps);  
           assert step.MaybeAcceptStep?;
-          assert acceptedVal == v'.History(i).leaders[ldr].value;
+          assert acceptedVal == v'.History(i).leaders[ldr].Value();
         }
       } else if dsStep.LeaderStep? {
         NotAcceptorStepImpliesNoPromiseOrAccept(c,  v.Last(), v'.Last(), v.network, v'.network, dsStep);
@@ -624,7 +622,7 @@ lemma InvNextLearnerReceivedAcceptImpliesProposed(c: Constants, v: Variables, v'
   requires v.WF(c)
   requires ValidMessageSrc(c, v)
   requires SendAcceptValidity(c, v)
-  requires LeaderCanProposeVMonotonic(c, v)
+  requires LeaderReceivedPromisesAndValueMonotonic(c, v)
   requires LearnerValidReceivedAcceptsKeys(c, v)
   requires AcceptorValidPromisedAndAccepted(c, v)
   requires AcceptorAcceptedImpliesProposed(c, v)
@@ -663,7 +661,7 @@ lemma InvNextAcceptorAcceptedImpliesProposed(c: Constants, v: Variables, v': Var
   requires v.WF(c)
   requires ValidMessageSrc(c, v)
   requires SendProposeValidity(c, v)
-  requires LeaderCanProposeVMonotonic(c, v)
+  requires LeaderReceivedPromisesAndValueMonotonic(c, v)
   requires AcceptorValidPromisedAndAccepted(c, v)
   requires AcceptorAcceptedImpliesProposed(c, v)
   requires Next(c, v, v')
@@ -726,7 +724,7 @@ lemma InvNextLeaderHearedImpliesProposed(c: Constants, v: Variables, v': Variabl
     var b := vi'.leaders[ldr].highestHeardBallot.value;
     && c.ValidLeaderIdx(b)
     && vi'.LeaderCanPropose(c, b)
-    && vi'.leaders[b].value == vi'.leaders[ldr].value
+    && vi'.leaders[b].Value() == vi'.leaders[ldr].Value()
   { 
     VariableNextProperties(c, v, v');
     if i == |v'.history| - 1 {
@@ -756,7 +754,7 @@ lemma InvNextLeaderReceivedPromisesImpliesAcceptorState(c: Constants, v: Variabl
     && v'.ValidHistoryIdx(i)
     && c.ValidLeaderIdx(ldr)
     && c.ValidAcceptorIdx(acc)
-    && acc in v'.History(i).leaders[ldr].receivedPromises.s
+    && acc in v'.History(i).leaders[ldr].ReceivedPromises()
   ensures
     v'.History(i).acceptors[acc].HasPromisedAtLeast(ldr)
   {
@@ -802,7 +800,7 @@ lemma InvNextLeaderHighestHeardToPromisedRangeHasNoAccepts(c: Constants, v: Vari
     && vb in v'.History(i).learners[lnr].receivedAccepts.m
     && vb.b < ldr
     && v'.History(i).leaders[ldr].HeardAtMost(vb.b)
-    && acc in v'.History(i).leaders[ldr].receivedPromises.s
+    && acc in v'.History(i).leaders[ldr].ReceivedPromises()
   ensures
     acc !in v'.History(i).learners[lnr].receivedAccepts.m[vb]
   {
@@ -957,7 +955,7 @@ lemma InvNextChosenValImpliesLeaderOnlyHearsVal(c: Constants, v: Variables, v': 
     && c.ValidLeaderIdx(ldrBal)
     && v'.History(i).leaders[ldrBal].HeardAtLeast(vb.b)
   ensures
-    v'.History(i).leaders[ldrBal].value == vb.v
+    v'.History(i).leaders[ldrBal].Value() == vb.v
   {
     VariableNextProperties(c, v, v');
     if i == |v'.history| - 1 {
@@ -970,7 +968,7 @@ lemma InvNextChosenValImpliesLeaderOnlyHearsVal(c: Constants, v: Variables, v': 
       } else if dsStep.AcceptorStep? {
         NewChosenOnlyInLearnerStep(c, v, v', dsStep);
       } else {
-        if v'.History(i).leaders[ldrBal].value != vb.v {
+        if v'.History(i).leaders[ldrBal].Value() != vb.v {
           assert Chosen(c, v', vb) by {
             reveal_Chosen();
           }
@@ -1051,10 +1049,10 @@ lemma InvNextChosenImpliesProposingLeaderHearsChosenBallotLeaderStep(
       var acc := dsStep.msgOps.recv.value.acc;
       if acc !in choosingAccs {
         // In this case, by quorum intersection, acc must already be in ldr.receivePromises
-        // Because, choosingAccs !! v.leaders[ldr].receivedPromises.s
+        // Because, choosingAccs !! v.leaders[ldr].ReceivedPromises()
         reveal_ValidMessageSrc();
         var allAccs := GetAcceptorSet(c, v);
-        var e := QuorumIntersection(allAccs, choosingAccs, h.leaders[ldr].receivedPromises.s + {acc});
+        var e := QuorumIntersection(allAccs, choosingAccs, h.leaders[ldr].ReceivedPromises() + {acc});
         assert false;
       }      
     }    
@@ -1092,7 +1090,7 @@ lemma InvNextChosenImpliesProposingLeaderHearsChosenBallotLearnerStep(
       assert v.Last().LeaderCanPropose(c, ldr);  // trigger
       if !v.Last().leaders[ldr].HeardAtLeast(vb.b) {
         var allAccs := GetAcceptorSet(c, v);
-        var e := QuorumIntersection(allAccs, choosingAccs, v.Last().leaders[ldr].receivedPromises.s);
+        var e := QuorumIntersection(allAccs, choosingAccs, v.Last().leaders[ldr].ReceivedPromises());
         assert false;
       } 
     } else {
@@ -1107,7 +1105,7 @@ lemma LeaderHearsDifferentValueFromChosenImpliesFalse(c: Constants, v: Variables
   requires Chosen(c, v, chosen)
   requires c.ValidLeaderIdx(ldr)
   requires v.Last().leaders[ldr].HeardAtLeast(chosen.b)
-  requires v.Last().leaders[ldr].value != chosen.v
+  requires v.Last().leaders[ldr].Value() != chosen.v
   requires chosen.b < ldr
   requires OneValuePerBallot(c, v)
   requires LeaderHighestHeardUpperBound(c, v)
@@ -1121,7 +1119,7 @@ lemma LeaderHearsDifferentValueFromChosenImpliesFalse(c: Constants, v: Variables
     Then do recursion all the way down.
   */
   var ldr' := v.Last().leaders[ldr].highestHeardBallot.value;
-  assert v.Last().leaders[ldr'].value == v.Last().leaders[ldr].value;
+  assert v.Last().leaders[ldr'].Value() == v.Last().leaders[ldr].Value();
   assert chosen.b <= ldr' < ldr;
   reveal_Chosen();
   reveal_ChosenAtHistory();
@@ -1361,8 +1359,7 @@ lemma ChosenImpliesProposeMessagesOnlyContainValue(c: Constants, v: Variables, v
 
 lemma LeaderCanProposeMonotonicLemma(c: Constants, v: Variables)
   requires v.WF(c)
-  requires LeaderReceivedPromisesMonotonic(c, v)
-  requires LeaderCanProposeVMonotonic(c, v)
+  requires LeaderReceivedPromisesAndValueMonotonic(c, v)
   ensures forall i, j, ldr |
     && v.ValidHistoryIdx(i)
     && v.ValidHistoryIdx(j)
@@ -1371,24 +1368,6 @@ lemma LeaderCanProposeMonotonicLemma(c: Constants, v: Variables)
     && v.History(i).LeaderCanPropose(c, ldr)
   :: 
     && v.History(j).LeaderCanPropose(c, ldr)
-    && v.History(j).leaders[ldr].value == v.History(i).leaders[ldr].value
-{
-  // forall i, j, ldr |
-  //   && v.ValidHistoryIdx(i)
-  //   && v.ValidHistoryIdx(j)
-  //   && i <= j
-  //   && c.ValidLeaderIdx(ldr)
-  //   && v.History(i).LeaderCanPropose(c, ldr)
-  // ensures
-  //   && v.History(j).LeaderCanPropose(c, ldr)
-  //   && v.History(j).leaders[ldr].value == v.History(i).leaders[ldr].value
-  // {
-  //   var lc := c.leaderConstants[ldr];
-  //   // SetContainmentCardinality(v.History(i).leaders[ldr].receivedPromises.s, v.History(j).leaders[ldr].receivedPromises.s);
-  //   // var val := v.History(j).leaders[ldr].value;
-  //   // assert v.History(i).leaders[ldr].MonotonicCanProposeV(lc, val);
-  
-  //   // assert v.History(j).leaders[ldr].value == v.History(i).leaders[ldr].value;
-  // }
-}
+    && v.History(j).leaders[ldr].Value() == v.History(i).leaders[ldr].Value()
+{}
 } // end module PaxosProof
